RingBuffer/example1_ddl.thy
@@ -1,25 +1,6 @@
 theory example1_ddl 
-	imports "HOLCF-Library.Nat_Discrete" "HOLCF-Library.Int_Discrete"
-          "HOLCF-Library.List_Cpo"  DeadlockFreedom_Automation Law_Interrupt_Seq  (*Example1_ddlf_no_final can not be imported, why?*)
+	imports  DeadlockFreedom  (*Example1_ddlf_no_final can not be imported, why?*)
 begin
-
-default_sort type
-
-
-no_notation floor (\<open>\<lfloor>_\<rfloor>\<close>)
-no_notation ceiling (\<open>\<lceil>_\<rceil>\<close>)
-
-no_notation Cons  ("_ \<cdot>/ _" [66,65] 65)
-
-abbreviation "dot"    :: "['a \<Rightarrow> 'b, 'a, 'b process] \<Rightarrow> 'b process"
-  where      "dot c
- a P \<equiv> write c a P"
-
-syntax   "_dot"  :: "[id, logic, 'a process] => 'a process"
-                                        ("(3(_\<^bold>._) /\<rightarrow> _)" [0,0,78] 78)
-translations
- 
-  "_dot c p P"     \<rightleftharpoons> "CONST dot c p P"
 
 
 subsection \<open> Model \<close>
@@ -145,7 +126,7 @@ where
 
 
 lemma SSTOP_nonTerm: \<open>non_terminating SSTOP\<close>
-  by (metis AfterExt.deadlock_free_iff_empty_ticks_of_and_deadlock_free\<^sub>S\<^sub>K\<^sub>I\<^sub>P\<^sub>S Trans.SSTOP.unfold ex1_m' non_terminating_is_empty_ticks_of)
+  by (metis AfterExt.deadlock_free_iff_empty_ticks_of_and_deadlock_free\<^sub>S\<^sub>K\<^sub>I\<^sub>P\<^sub>S Trans.SSTOP.unfold prefix_recursive_ddlf non_terminating_is_empty_ticks_of)
 
 lemma prefix_Skip_no_initial_tick : \<open> (a\<rightarrow> Skip)\<^sup>0 \<inter> range tick = {}\<close>
   by (simp add: image_iff initials_write0)
@@ -252,7 +233,7 @@ lemma Trans_stm0_core'_ddlf:
  (*  apply (auto intro!:prefix_proving_Mndetprefix_UNIV_ref(3)
   eat_lemma no_step_refine generalized_refine_guarded_extchoice write_proving_Mndetprefix_UNIV_ref GlobalNdet_refine_no_step )
 *)
-  sledgehammer
+  
 (*the guard can not be discharged*)
   nitpick
   oops
@@ -276,8 +257,6 @@ lemma Trans_stm0_core'_ddlf_auto:
 
 
 end
-thm Trans.Trans_stm0_core_def
-term "Trans.Trans_stm0_core"
 end
 
 
